Auto/Embedding/LamPrep.lean
@@ -18,7 +18,13 @@ theorem LamEquiv.not_true_equiv_false :
   LamEquiv lval lctx (.base .prop) (.mkNot (.base .trueE)) (.base .falseE) := by
   exists LamWF.mkNot (.ofBase .ofTrueE); exists LamWF.ofBase .ofFalseE; intro lctxTerm
   dsimp [LamWF.interp, LamBaseTerm.LamWF.interp, notLift]
-  apply GLift.down.inj; dsimp; apply eq_false; exact fun h => (h .intro)
+  apply GLift.down.inj; dsimp; apply eq_false; exact fun h => h .intro
+
+theorem LamEquiv.not_false_equiv_true :
+  LamEquiv lval lctx (.base .prop) (.mkNot (.base .falseE)) (.base .trueE) := by
+  exists LamWF.mkNot (.ofBase .ofFalseE); exists LamWF.ofBase .ofTrueE; intro lctxTerm
+  dsimp [LamWF.interp, LamBaseTerm.LamWF.interp, notLift]
+  apply GLift.down.inj; dsimp; apply eq_true; exact id
 
 theorem LamEquiv.prop_ne_equiv_eq_not
   (wfl : LamWF lval.toLamTyVal ⟨lctx, lhs, .base .prop⟩)
@@ -34,8 +40,38 @@ theorem LamEquiv.prop_ne_equiv_eq_not
     intro h h'; have h' := _root_.congrArg GLift.down h'; revert h'
     apply ne_of_eq_not; dsimp at h; rw [h]
 
+-- (a ≠ b) ↔ (a = (¬ b))
+def LamTerm.prop_ne_equiv_eq_not? (t : LamTerm) : Option LamTerm :=
+  match t with
+  | .app _ (.base .not) (.app _ (.app _ (.base (.eq (.base .prop))) lhs) rhs) =>
+    .some (.mkEq (.base .prop) lhs (.mkNot rhs))
+  | _ => .none
+
+theorem LamTerm.maxEVarSucc_prop_ne_equiv_eq_not?
+  (heq : prop_ne_equiv_eq_not? t = .some t') : t'.maxEVarSucc = t.maxEVarSucc :=
+  match t, heq with
+  | .app _ (.base .not) (.app _ (.app _ (.base (.eq (.base .prop))) lhs) rhs), Eq.refl _ => by
+    dsimp [maxEVarSucc]; simp [Nat.max, Nat.max_zero_left, Nat.max_zero_right]
+
+theorem LamEquiv.prop_ne_equiv_eq_not?
+  (wft : LamWF lval.toLamTyVal ⟨lctx, t, s⟩)
+  (heq : LamTerm.prop_ne_equiv_eq_not? t = .some t') :
+  LamEquiv lval lctx (.base .prop) t t' :=
+  match t, heq with
+  | .app _ (.base .not) (.app _ (.app _ (.base (.eq (.base .prop))) lhs) rhs), Eq.refl _ => by
+    cases wft.getFn.getBase; cases wft.getArg.getFn.getFn.getBase
+    match wft with
+    | .ofApp _ (.ofBase .ofNot) (.ofApp _ (.ofApp _ (.ofBase (.ofEq _)) Hlhs) Hrhs) =>
+      apply LamEquiv.prop_ne_equiv_eq_not Hlhs Hrhs
+
+theorem LamThmEquiv.prop_ne_equiv_eq_not?
+  (wft : LamThmWF lval lctx s t)
+  (heq : LamTerm.prop_ne_equiv_eq_not? t = .some t') :
+  LamThmEquiv lval lctx (.base .prop) t t' :=
+  fun lctx' => LamEquiv.prop_ne_equiv_eq_not? (wft lctx') heq
+
 theorem LamTerm.maxEVarSucc_equalize : (LamTerm.equalize t).maxEVarSucc = t.maxEVarSucc := by
-  dsimp [maxEVarSucc]; simp [Nat.max, Nat.max_zero_left, Nat.max_zero_right]
+  simp [maxEVarSucc, Nat.max, Nat.max_zero_left, Nat.max_zero_right]
 
 theorem LamEquiv.equalize (wft : LamWF lval.toLamTyVal ⟨lctx, t, .base .prop⟩) :
   LamEquiv lval lctx (.base .prop) t t.equalize := by
@@ -49,6 +85,7 @@ theorem LamThmEquiv.equalize (wft : LamThmWF lval lctx (.base .prop) t) :
   LamThmEquiv lval lctx (.base .prop) t t.equalize :=
   fun lctx' => LamEquiv.equalize (wft lctx')
 
+-- (True = False) ↔ False
 def LamTerm.true_eq_false_equiv_false? (t : LamTerm) : Option LamTerm :=
   match t.beq (.mkEq (.base .prop) (.base .trueE) (.base .falseE)) with
   | true => .some (.base .falseE)
@@ -90,6 +127,7 @@ theorem LamThmEquiv.true_eq_false_equiv_false?
   LamThmEquiv lval lctx (.base .prop) t t' :=
   fun lctx' => LamEquiv.true_eq_false_equiv_false? (wft lctx') heq
 
+-- (False = True) ↔ False
 def LamTerm.false_eq_true_equiv_false? (t : LamTerm) : Option LamTerm :=
   match t.beq (.mkEq (.base .prop) (.base .falseE) (.base .trueE)) with
   | true => .some (.base .falseE)
@@ -131,6 +169,79 @@ theorem LamThmEquiv.false_eq_true_equiv_false?
   LamThmEquiv lval lctx (.base .prop) t t' :=
   fun lctx' => LamEquiv.false_eq_true_equiv_false? (wft lctx') heq
 
+-- (a = True) ↔ a
+def LamTerm.eq_true_equiv? (t : LamTerm) : Option LamTerm :=
+  match t with
+  | .app _ (.app _ (.base (.eq _)) lhs) (.base .trueE) => .some lhs
+  | _ => .none
+
+theorem LamTerm.maxEVarSucc_eq_true_equiv?
+  (heq : LamTerm.eq_true_equiv? t = .some t') :
+  t'.maxEVarSucc = t.maxEVarSucc :=
+  match t, heq with
+  | .app _ (.app _ (.base (.eq _)) lhs) (.base .trueE), Eq.refl _ => by
+    simp [maxEVarSucc, Nat.max, Nat.max_zero_left, Nat.max_zero_right]
+
+theorem LamEquiv.eq_true_equiv?
+  (wft : LamWF lval.toLamTyVal ⟨lctx, t, s⟩)
+  (heq : LamTerm.eq_true_equiv? t = .some t') :
+  LamEquiv lval lctx (.base .prop) t t' :=
+  match t, heq with
+  | .app _ (.app _ (.base (.eq _)) lhs) (.base .trueE), Eq.refl _ => by
+    cases wft.getFn.getFn.getBase; cases wft.getArg.getBase; exists wft
+    match wft with
+    | .ofApp _ (.ofApp _ (.ofBase (.ofEq _)) Hlhs) (.ofBase .ofTrueE) =>
+      exists Hlhs; intro lctxTerm
+      dsimp [LamWF.interp, LamBaseTerm.LamWF.interp, eqLiftFn]
+      apply GLift.down.inj; dsimp; apply propext (Iff.intro ?mp ?mpr)
+      case mp =>
+        intro h; apply of_eq_true (_root_.congrArg _ h)
+      case mpr =>
+        intro h; apply GLift.down.inj _ _ (eq_true h)
+
+theorem LamThmEquiv.eq_true_equiv?
+  (wft : LamThmWF lval lctx s t)
+  (heq : LamTerm.eq_true_equiv? t = .some t') :
+  LamThmEquiv lval lctx (.base .prop) t t' :=
+  fun lctx' => LamEquiv.eq_true_equiv? (wft lctx') heq
+
+-- (a = False) ↔ (¬ a)
+def LamTerm.eq_false_equiv? (t : LamTerm) : Option LamTerm :=
+  match t with
+  | .app _ (.app _ (.base (.eq _)) lhs) (.base .falseE) => .some (.mkNot lhs)
+  | _ => .none
+
+theorem LamTerm.maxEVarSucc_eq_false_equiv?
+  (heq : LamTerm.eq_false_equiv? t = .some t') :
+  t'.maxEVarSucc = t.maxEVarSucc :=
+  match t, heq with
+  | .app _ (.app _ (.base (.eq _)) lhs) (.base .falseE), Eq.refl _ => by
+    simp [maxEVarSucc, Nat.max, Nat.max_zero_left, Nat.max_zero_right]
+
+theorem LamEquiv.eq_false_equiv?
+  (wft : LamWF lval.toLamTyVal ⟨lctx, t, s⟩)
+  (heq : LamTerm.eq_false_equiv? t = .some t') :
+  LamEquiv lval lctx (.base .prop) t t' :=
+  match t, heq with
+  | .app _ (.app _ (.base (.eq _)) lhs) (.base .falseE), Eq.refl _ => by
+    cases wft.getFn.getFn.getBase; cases wft.getArg.getBase; exists wft
+    match wft with
+    | .ofApp _ (.ofApp _ (.ofBase (.ofEq _)) Hlhs) (.ofBase .ofFalseE) =>
+      exists LamWF.mkNot Hlhs; intro lctxTerm
+      dsimp [LamWF.interp, LamBaseTerm.LamWF.interp, eqLiftFn]
+      apply GLift.down.inj; dsimp; apply propext (Iff.intro ?mp ?mpr)
+      case mp =>
+        intro h h'; rw [h] at h'; exact h'
+      case mpr =>
+        intro h; apply GLift.down.inj _ _ (eq_false h)
+
+theorem LamThmEquiv.eq_false_equiv?
+  (wft : LamThmWF lval lctx s t)
+  (heq : LamTerm.eq_false_equiv? t = .some t') :
+  LamThmEquiv lval lctx (.base .prop) t t' :=
+  fun lctx' => LamEquiv.eq_false_equiv? (wft lctx') heq
+
+-- (a ≠ True) ↔ (a = False)
 def LamTerm.ne_true_equiv_eq_false? (t : LamTerm) : Option LamTerm :=
   match t with
   | .app _ (.base .not) (.app s (.app _ (.base (.eq _)) lhs) (.base .trueE)) =>
@@ -139,53 +250,232 @@ def LamTerm.ne_true_equiv_eq_false? (t : LamTerm) : Option LamTerm :=
 
 theorem LamTerm.maxEVarSucc_ne_true_equiv_eq_false?
   (heq : LamTerm.ne_true_equiv_eq_false? t = .some t') :
-  t'.maxEVarSucc = t.maxEVarSucc := by
-  cases t <;> try cases heq
-  case app s fn arg =>
-    cases fn <;> try cases heq
-    case base b =>
-      cases b <;> try cases heq
-      cases arg <;> try cases heq
-      case app _ fn arg =>
-        cases fn <;> try cases heq
-        case app _ fn' arg' =>
-          cases fn' <;> try cases heq
-          case base b =>
-            cases b <;> try cases heq
-            cases arg <;> try cases heq
-            case base b =>
-              cases b <;> try cases heq
-              simp [maxEVarSucc, Nat.max]
-              simp [Nat.max_zero_left, Nat.max_zero_right]
+  t'.maxEVarSucc = t.maxEVarSucc :=
+  match t, heq with
+  | .app _ (.base .not) (.app _ (.app _ (.base (.eq _)) lhs) (.base .trueE)), Eq.refl _ => by
+    simp [maxEVarSucc, Nat.max, Nat.max_zero_left, Nat.max_zero_right]
 
 theorem LamEquiv.ne_true_equiv_eq_false?
   (wft : LamWF lval.toLamTyVal ⟨lctx, t, s⟩)
   (heq : LamTerm.ne_true_equiv_eq_false? t = .some t') :
-  LamEquiv lval lctx (.base .prop) t t' := by
-  cases t <;> try cases heq
-  case app s fn arg =>
-    cases fn <;> try cases heq
-    case base b =>
-      cases b <;> try cases heq
-      cases wft.getFn.getBase
-      cases arg <;> try cases heq
-      case app _ fn arg =>
-        cases fn <;> try cases heq
-        case app _ fn' arg' =>
-          cases fn' <;> try cases heq
-          case base b =>
-            cases b <;> try cases heq
-            cases arg <;> try cases heq
-            case base b =>
-              cases b <;> try cases heq
-              match wft with
-              | .ofApp _ (.ofBase .ofNot) (.ofApp _ (.ofApp _ (.ofBase (.ofEq _)) Hlhs) (.ofBase .ofTrueE)) =>
-                apply LamEquiv.trans (prop_ne_equiv_eq_not Hlhs (.ofBase .ofTrueE))
-                apply LamEquiv.congrArg (.ofApp _ (.ofBase (.ofEq _)) Hlhs)
-                apply LamEquiv.not_true_equiv_false
+  LamEquiv lval lctx (.base .prop) t t' :=
+  match t, heq with
+  | .app _ (.base .not) (.app _ (.app _ (.base (.eq _)) lhs) (.base .trueE)), Eq.refl _ =>
+    match wft with
+    | .ofApp _ (.ofBase .ofNot) (.ofApp _ (.ofApp _ (.ofBase (.ofEq _)) Hlhs) (.ofBase .ofTrueE)) => by
+      apply LamEquiv.trans (prop_ne_equiv_eq_not Hlhs (.ofBase .ofTrueE))
+      apply LamEquiv.congrArg (.ofApp _ (.ofBase (.ofEq _)) Hlhs)
+      apply LamEquiv.not_true_equiv_false
 
 theorem LamThmEquiv.ne_true_equiv_eq_false?
   (wft : LamThmWF lval lctx s t)
   (heq : LamTerm.ne_true_equiv_eq_false? t = .some t') :
   LamThmEquiv lval lctx (.base .prop) t t' :=
   fun lctx' => LamEquiv.ne_true_equiv_eq_false? (wft lctx') heq
+
+-- (a ≠ False) ↔ (a = True)
+def LamTerm.ne_false_equiv_eq_true? (t : LamTerm) : Option LamTerm :=
+  match t with
+  | .app _ (.base .not) (.app s (.app _ (.base (.eq _)) lhs) (.base .falseE)) =>
+    .some (.app s (.app s (.base (.eq s)) lhs) (.base .trueE))
+  | _ => .none
+
+theorem LamTerm.maxEVarSucc_ne_false_equiv_eq_true?
+  (heq : LamTerm.ne_false_equiv_eq_true? t = .some t') :
+  t'.maxEVarSucc = t.maxEVarSucc :=
+  match t, heq with
+  | .app _ (.base .not) (.app _ (.app _ (.base (.eq _)) lhs) (.base .falseE)), Eq.refl _ => by
+    simp [maxEVarSucc, Nat.max, Nat.max_zero_left, Nat.max_zero_right]
+
+theorem LamEquiv.ne_false_equiv_eq_true?
+  (wft : LamWF lval.toLamTyVal ⟨lctx, t, s⟩)
+  (heq : LamTerm.ne_false_equiv_eq_true? t = .some t') :
+  LamEquiv lval lctx (.base .prop) t t' :=
+  match t, heq with
+  | .app _ (.base .not) (.app _ (.app _ (.base (.eq _)) lhs) (.base .falseE)), Eq.refl _ =>
+    match wft with
+    | .ofApp _ (.ofBase .ofNot) (.ofApp _ (.ofApp _ (.ofBase (.ofEq _)) Hlhs) (.ofBase .ofFalseE)) => by
+      apply LamEquiv.trans (prop_ne_equiv_eq_not Hlhs (.ofBase .ofFalseE))
+      apply LamEquiv.congrArg (.ofApp _ (.ofBase (.ofEq _)) Hlhs)
+      apply LamEquiv.not_false_equiv_true
+
+theorem LamThmEquiv.ne_false_equiv_eq_true?
+  (wft : LamThmWF lval lctx s t)
+  (heq : LamTerm.ne_false_equiv_eq_true? t = .some t') :
+  LamThmEquiv lval lctx (.base .prop) t t' :=
+  fun lctx' => LamEquiv.ne_false_equiv_eq_true? (wft lctx') heq
+
+-- ((¬ a) = True) ↔ (a = False)
+def LamTerm.not_eq_true_equiv_eq_false? (t : LamTerm) : Option LamTerm :=
+  match t with
+  | .app _ (.app _ (.base (.eq _)) (.app _ (.base .not) lhs)) (.base .trueE) =>
+    .some (.mkEq (.base .prop) lhs (.base .falseE))
+  | _ => .none
+
+def LamTerm.maxEVarSucc_not_eq_true_equiv_eq_false?
+  (heq : LamTerm.not_eq_true_equiv_eq_false? t = .some t') :
+  t'.maxEVarSucc = t.maxEVarSucc :=
+  match t, heq with
+  | .app _ (.app _ (.base (.eq _)) (.app _ (.base .not) lhs)) (.base .trueE), Eq.refl _ => by
+    simp [maxEVarSucc, Nat.max, Nat.max_zero_left]
+
+theorem LamEquiv.not_eq_true_equiv_eq_false?
+  (wft : LamWF lval.toLamTyVal ⟨lctx, t, s⟩)
+  (heq : LamTerm.not_eq_true_equiv_eq_false? t = .some t') :
+  LamEquiv lval lctx (.base .prop) t t' :=
+  match t, heq with
+  | .app _ (.app _ (.base (.eq _)) (.app _ (.base .not) lhs)) (.base .trueE), Eq.refl _ => by
+    cases wft.getFn.getFn.getBase; cases wft.getFn.getArg.getFn.getBase
+    match wft with
+    | .ofApp _ (.ofApp _ (.ofBase (.ofEq _)) (.ofApp _ (.ofBase .ofNot) Hlhs)) (.ofBase .ofTrueE) =>
+      apply trans (eqSymm? wft rfl)
+      apply trans (symm (prop_ne_equiv_eq_not (.ofBase .ofTrueE) Hlhs))
+      apply trans _ (ne_true_equiv_eq_false? (LamWF.mkNot (.mkEq Hlhs (.ofBase .ofTrueE))) rfl)
+      apply congrArg (.ofBase .ofNot); apply eqSymm? (.mkEq (.ofBase .ofTrueE) Hlhs) rfl
+
+theorem LamThmEquiv.not_eq_true_equiv_eq_false?
+  (wft : LamThmWF lval lctx s t)
+  (heq : LamTerm.not_eq_true_equiv_eq_false? t = .some t') :
+  LamThmEquiv lval lctx (.base .prop) t t' :=
+  fun lctx' => LamEquiv.not_eq_true_equiv_eq_false? (wft lctx') heq
+
+def LamTerm.not_eq_false_equiv_eq_true? (t : LamTerm) : Option LamTerm :=
+  match t with
+  | .app _ (.app _ (.base (.eq _)) (.app _ (.base .not) lhs)) (.base .falseE) =>
+    .some (.mkEq (.base .prop) lhs (.base .trueE))
+  | _ => .none
+
+def LamTerm.maxEVarSucc_not_eq_false_equiv_eq_true?
+  (heq : LamTerm.not_eq_false_equiv_eq_true? t = .some t') :
+  t'.maxEVarSucc = t.maxEVarSucc :=
+  match t, heq with
+  | .app _ (.app _ (.base (.eq _)) (.app _ (.base .not) lhs)) (.base .falseE), Eq.refl _ => by
+    simp [maxEVarSucc, Nat.max, Nat.max_zero_left]
+
+theorem LamEquiv.not_eq_false_equiv_eq_true?
+  (wft : LamWF lval.toLamTyVal ⟨lctx, t, s⟩)
+  (heq : LamTerm.not_eq_false_equiv_eq_true? t = .some t') :
+  LamEquiv lval lctx (.base .prop) t t' :=
+  match t, heq with
+  | .app _ (.app _ (.base (.eq _)) (.app _ (.base .not) lhs)) (.base .falseE), Eq.refl _ => by
+    cases wft.getFn.getFn.getBase; cases wft.getFn.getArg.getFn.getBase
+    match wft with
+    | .ofApp _ (.ofApp _ (.ofBase (.ofEq _)) (.ofApp _ (.ofBase .ofNot) Hlhs)) (.ofBase .ofFalseE) =>
+      apply trans (eqSymm? wft rfl)
+      apply trans (symm (prop_ne_equiv_eq_not (.ofBase .ofFalseE) Hlhs))
+      apply trans _ (ne_false_equiv_eq_true? (LamWF.mkNot (.mkEq Hlhs (.ofBase .ofFalseE))) rfl)
+      apply congrArg (.ofBase .ofNot); apply eqSymm? (.mkEq (.ofBase .ofFalseE) Hlhs) rfl
+
+theorem LamThmEquiv.not_eq_false_equiv_eq_true?
+  (wft : LamThmWF lval lctx s t)
+  (heq : LamTerm.not_eq_false_equiv_eq_true? t = .some t') :
+  LamThmEquiv lval lctx (.base .prop) t t' :=
+  fun lctx' => LamEquiv.not_eq_false_equiv_eq_true? (wft lctx') heq
+
+-- (¬¬a) ↔ a
+theorem LamEquiv.not_not_equiv
+  (wft : LamWF lval.toLamTyVal ⟨lctx, t, .base .prop⟩) :
+  LamEquiv lval lctx (.base .prop) (.mkNot (.mkNot t)) t := by
+  exists (.mkNot (.mkNot wft)); exists wft; intro lctxTerm
+  dsimp [LamWF.interp, LamBaseTerm.LamWF.interp, notLift]
+  apply GLift.down.inj; dsimp
+  apply propext (Iff.intro Classical.byContradiction (fun a b => b a))
+
+theorem LamThmEquiv.not_not_equiv
+  (wft : LamThmWF lval lctx (.base .prop) t) :
+  LamThmEquiv lval lctx (.base .prop) (.mkNot (.mkNot t)) t :=
+  fun lctx' => LamEquiv.not_not_equiv (wft lctx')
+
+-- ((¬ a) = b) ↔ (a = (¬ b))
+def LamTerm.not_eq_equiv_eq_not? (t : LamTerm) : Option LamTerm :=
+  match t with
+  | .app _ (.app _ (.base (.eq _)) (.app _ (.base .not) lhs)) rhs =>
+    .some (.mkEq (.base .prop) lhs (.mkNot rhs))
+  | _ => .none
+
+theorem LamTerm.maxEVarSucc_not_eq_equiv_eq_not?
+  (heq : LamTerm.not_eq_equiv_eq_not? t = .some t') :
+  t.maxEVarSucc = t'.maxEVarSucc :=
+  match t, heq with
+  | .app _ (.app _ (.base (.eq _)) (.app _ (.base .not) lhs)) rhs, Eq.refl _ => by
+    simp [maxEVarSucc, Nat.max, Nat.max_zero_left]
+
+theorem LamEquiv.not_eq_equiv_eq_not?
+  (wft : LamWF lval.toLamTyVal ⟨lctx, t, s⟩)
+  (heq : LamTerm.not_eq_equiv_eq_not? t = .some t') :
+  LamEquiv lval lctx (.base .prop) t t' :=
+  match t, heq with
+  | .app _ (.app _ (.base (.eq _)) (.app _ (.base .not) lhs)) rhs, Eq.refl _ => by
+    cases wft.getFn.getFn.getBase; cases wft.getFn.getArg.getFn.getBase
+    match wft with
+    | .ofApp _ (.ofApp _ (.ofBase (.ofEq _)) (.ofApp _ (.ofBase .ofNot) Hlhs)) Hrhs =>
+      apply trans (eqSymm? (.mkEq (.mkNot Hlhs) Hrhs) rfl) (trans _ (prop_ne_equiv_eq_not Hlhs Hrhs))
+      apply trans (symm (prop_ne_equiv_eq_not Hrhs Hlhs)) (neSymm? (.mkNot (.mkEq Hrhs Hlhs)) rfl)
+
+-- ((¬ a) = (¬ b)) ↔ (a = b)
+def LamTerm.not_eq_not_equiv_eq? (t : LamTerm) : Option LamTerm :=
+  match t with
+  | .app _ (.app _ (.base (.eq _)) (.app _ (.base .not) lhs)) (.app _ (.base .not) rhs) =>
+    .some (.mkEq (.base .prop) lhs rhs)
+  | _ => .none
+
+theorem LamTerm.maxEVarSucc_not_eq_not_equiv_eq?
+  (heq : LamTerm.not_eq_not_equiv_eq? t = .some t') :
+  t.maxEVarSucc = t'.maxEVarSucc :=
+  match t, heq with
+  | .app _ (.app _ (.base (.eq _)) (.app _ (.base .not) lhs)) (.app _ (.base .not) rhs), Eq.refl _ => by
+    simp [maxEVarSucc, Nat.max, Nat.max_zero_left]
+
+theorem LamEquiv.not_eq_not_equiv_eq?
+  (wft : LamWF lval.toLamTyVal ⟨lctx, t, s⟩)
+  (heq : LamTerm.not_eq_not_equiv_eq? t = .some t') :
+  LamEquiv lval lctx (.base .prop) t t' :=
+  match t, heq with
+  | .app _ (.app _ (.base (.eq _)) (.app _ (.base .not) lhs)) (.app _ (.base .not) rhs), Eq.refl _ => by
+    cases wft.getFn.getFn.getBase; cases wft.getArg.getFn.getBase; cases wft.getFn.getArg.getFn.getBase
+    match wft with
+    | .ofApp _ (.ofApp _ (.ofBase (.ofEq _)) (.ofApp _ (.ofBase .ofNot) Hlhs)) (.ofApp _ (.ofBase .ofNot) Hrhs) =>
+      apply trans (symm (not_eq_equiv_eq_not? (.mkEq (.mkNot (.mkNot Hlhs)) Hrhs) rfl))
+      apply congrFun (congrArg (.ofBase (.ofEq _)) (not_not_equiv Hlhs)) Hrhs
+
+theorem LamThmEquiv.not_eq_not_equiv_eq?
+  (wft : LamThmWF lval lctx s t)
+  (heq : LamTerm.not_eq_not_equiv_eq? t = .some t') :
+  LamThmEquiv lval lctx (.base .prop) t t' :=
+  fun lctx' => LamEquiv.not_eq_not_equiv_eq? (wft lctx') heq
+
+-- (a ↔ b) ↔ (a = b)
+def LamTerm.iff_equiv_eq? (t : LamTerm) : Option LamTerm :=
+  match t with
+  | .app _ (.app _ (.base .iff) lhs) rhs => .some (.mkEq (.base .prop) lhs rhs)
+  | _ => .none
+
+theorem LamTerm.maxEVarSucc_iff_equiv_eq?
+  (heq : LamTerm.iff_equiv_eq? t = .some t') :
+  t.maxEVarSucc = t'.maxEVarSucc :=
+  match t, heq with
+  | .app _ (.app _ (.base .iff) lhs) rhs, Eq.refl _ => by
+    simp [maxEVarSucc, Nat.max, Nat.max_zero_left]
+
+theorem LamEquiv.iff_equiv_eq?
+  (wft : LamWF lval.toLamTyVal ⟨lctx, t, s⟩)
+  (heq : LamTerm.iff_equiv_eq?  t = .some t') :
+  LamEquiv lval lctx (.base .prop) t t' :=
+  match t, heq with
+  | .app _ (.app _ (.base .iff) lhs) rhs, Eq.refl _ => by
+    cases wft.getFn.getFn.getBase
+    match wft with
+    | .ofApp _ (.ofApp _ (.ofBase .ofIff) Hlhs) Hrhs =>
+      exists (.mkIff Hlhs Hrhs); exists (.mkEq Hlhs Hrhs); intro lctxTerm
+      dsimp [LamWF.interp, LamBaseTerm.LamWF.interp, iffLift, eqLiftFn]
+      apply GLift.down.inj; apply propext (Iff.intro ?mp ?mpr)
+      case mp =>
+        intro h; apply GLift.down.inj; apply propext h
+      case mpr =>
+        intro h; apply iff_of_eq (_root_.congrArg GLift.down h)
+
+theorem LamThmEquiv.iff_equiv_eq?
+  (wft : LamThmWF lval lctx s t)
+  (heq : LamTerm.iff_equiv_eq?  t = .some t') :
+  LamThmEquiv lval lctx (.base .prop) t t' :=
+  fun lctx' => LamEquiv.iff_equiv_eq? (wft lctx') heq
