Auto/Embedding/LamInference.lean
@@ -1,0 +1,190 @@
+import Auto.Embedding.LamSystem
+
+namespace Auto.Embedding.Lam
+
+def LamTerm.impApp? (t₁₂ t₁ : LamTerm) : Option LamTerm :=
+  match t₁₂ with
+  | .app _ (.app _ imp hyp) concl =>
+    match hyp.beq t₁ with
+    | true =>
+      match imp with
+      | .base b =>
+        match b with
+        | .imp => .some concl
+        | _ => .none
+      | _ => .none
+    | false => .none
+  | _ => .none
+
+theorem LamTerm.maxEVarSucc_impApp?
+  (heq : LamTerm.impApp? t₁₂ t₁ = .some t') : t'.maxEVarSucc ≤ t₁₂.maxEVarSucc := by
+  cases t₁₂ <;> try cases heq
+  case app s fn arg =>
+    cases fn <;> try cases heq
+    case app s' imp hyp =>
+      dsimp [impApp?] at heq
+      cases h : hyp.beq t₁
+      case true =>
+        rw [h] at heq; cases imp <;> try cases heq
+        case base b =>
+          cases b <;> try cases heq
+          dsimp [maxEVarSucc]; cases (LamTerm.eq_of_beq_eq_true h)
+          apply Nat.le_max_right
+      case false =>
+        rw [h] at heq; cases heq
+
+theorem LamValid.impApp
+  (v₁₂ : LamValid lval lctx t₁₂) (v₁ : LamValid lval lctx t₁)
+  (heq : LamTerm.impApp? t₁₂ t₁ = .some t₂) : LamValid lval lctx t₂ := by
+  dsimp [LamTerm.impApp?] at heq
+  cases t₁₂ <;> try cases heq
+  case app bp₁ hypimp concl =>
+    cases hypimp <;> try cases heq
+    case app bp₂ imp hyp =>
+      dsimp at heq
+      match h : LamTerm.beq hyp t₁ with
+      | true =>
+        rw [h] at heq
+        cases imp <;> try cases heq
+        case base b =>
+          cases b <;> cases heq
+          case imp =>
+            have ⟨wf₁₂, h₁₂⟩ := v₁₂
+            match wf₁₂ with
+            | .ofApp _ (.ofApp _ (.ofBase .ofImp) HArg) wfConcl =>
+              exists wfConcl; have ⟨wf₁, h₁⟩ := v₁;
+              intro lctxTerm; apply h₁₂; apply Eq.mp _ (h₁ lctxTerm);
+              apply congrArg; apply eq_of_heq; apply LamWF.interp_heq <;> try rfl
+              exact .symm (LamTerm.eq_of_beq_eq_true h)
+      | false =>
+        rw [h] at heq; cases heq
+
+theorem LamThmValid.impApp
+  (H₁₂ : LamThmValid lval lctx t₁₂) (H₁ : LamThmValid lval lctx t₁)
+  (heq : LamTerm.impApp? t₁₂ t₁ = .some res) : LamThmValid lval lctx res :=
+  fun lctx' => LamValid.impApp (H₁₂ lctx') (H₁ lctx') heq
+
+def LamTerm.impApps? (t : LamTerm) (ps : List LamTerm) : Option LamTerm :=
+  match ps with
+  | .nil => .some t
+  | .cons p ps =>
+    match t.impApp? p with
+    | .some t' => t'.impApps? ps
+    | .none => .none
+
+theorem LamTerm.maxEVarSucc_impApps?
+  (heq : LamTerm.impApps? t ps = .some t') : t'.maxEVarSucc ≤ t.maxEVarSucc := by
+  induction ps generalizing t t'
+  case nil => cases heq; apply Nat.le_refl
+  case cons p ps IH =>
+    dsimp [impApps?] at heq
+    match h : impApp? t p with
+    | .some t' =>
+      rw [h] at heq; dsimp at heq
+      apply Nat.le_trans (IH heq) (maxEVarSucc_impApp? h)
+    | .none => rw [h] at heq; cases heq
+
+theorem LamValid.impApps
+  (vt : LamValid lval lctx t) (vps : HList (LamValid lval lctx) ps)
+  (heq : LamTerm.impApps? t ps = .some t') : LamValid lval lctx t' := by
+  induction ps generalizing t
+  case nil => cases heq; exact vt
+  case cons head tail IH =>
+    match vps with
+    | .cons vHead vTail =>
+      dsimp [LamTerm.impApps?] at heq
+      match hap : LamTerm.impApp? t head with
+      | .some t'' =>
+        rw [hap] at heq; dsimp at heq
+        apply IH _ vTail heq
+        apply LamValid.impApp vt vHead hap
+      | .none => rw [hap] at heq; cases heq
+
+theorem LamThmValid.impApps
+  (vt : LamThmValid lval lctx t) (vps : HList (LamThmValid lval lctx) ps)
+  (heq : LamTerm.impApps? t ps = .some t') : LamThmValid lval lctx t' :=
+  fun lctx' => LamValid.impApps (vt lctx') (vps.map (fun _ tv => tv lctx')) heq
+
+theorem LamThmValid.define {lval : LamValuation.{u}}
+  (wft : LamThmWF lval [] s t) (heVar : t.maxEVarSucc ≤ eidx) :
+  ∃ val, LamThmValid (lval.insertEVarAt s val eidx) [] (.mkEq s (.etom eidx) t) := by
+  exists LamWF.interp lval dfLCtxTy (dfLCtxTerm _) (wft dfLCtxTy)
+  apply LamThmValid.ofLamThmValidD
+  let ltv₁ := lval.toLamTyVal
+  let ltv₂ := { lval.toLamTyVal with lamEVarTy := replaceAt s eidx lval.lamEVarTy}
+  have wft' := LamWF.eVarIrrelevance (ltv₁:=ltv₁) (ltv₂:=ltv₂) rfl rfl
+    (fun n H => LamTyVal.insertEVarAt_eVarIrrelevance (Nat.le_trans H heVar)) (wft dfLCtxTy)
+  apply And.intro
+  case left =>
+    rw [LamTerm.maxLooseBVarSucc_mkEq]; dsimp [LamTerm.maxLooseBVarSucc]
+    rw [Nat.max_zero_left]; have ⟨_, hlb⟩ := LamThmWFD.ofLamThmWF wft; apply hlb
+  case right =>
+    exists LamWF.mkEq LamWF.insertEVarAt_eIdx wft'
+    intro lctxTerm; dsimp [LamWF.interp, LamBaseTerm.LamWF.interp, eqLiftFn]
+    apply eq_of_heq; apply HEq.trans (LamWF.interp_insertEVarAt_eIdx _)
+    apply LamWF.interp_eVarIrrelevance <;> try rfl
+    intro n hn; apply LamValuation.insertEVarAt_eVarIrrelevance
+    apply Nat.le_trans hn heVar
+
+section Skolemization
+
+  def LamTerm.skolemize? (t : LamTerm) (eidx : Nat) (lctx : List LamSort) : Option (LamSort × LamTerm) :=
+    match t with
+    | .app _ (.base (.existE s)) p => .some (s, .app s p (LamTerm.bvarApps (.etom eidx) lctx 0))
+    | _ => .none
+
+  theorem LamTerm.maxEVarSucc_skolemize? (heq : LamTerm.skolemize? t eidx lctx = .some (s, t')) :
+    t'.maxEVarSucc ≤ max t.maxEVarSucc (.succ eidx) :=
+    match t, heq with
+    | .app _ (.base (.existE s)) p, Eq.refl _ => by
+      dsimp [maxEVarSucc]; rw [LamTerm.maxEVarSucc_bvarApps];
+      simp [Nat.max, Nat.max_zero_left]; apply Nat.le_refl
+  
+  theorem choose_spec' {p : α → β → Prop} (h : ∀ q, ∃ x, p x q) : ∃ (y : _ → _), ∀ q, p (y q) q :=
+    ⟨fun q => Classical.choose (h q), fun q => Classical.choose_spec (h q)⟩
+
+  theorem LamThmValid.skolemize
+    (vt : LamThmValid lval lctx (.mkExistE s p)) (heVar : p.maxEVarSucc ≤ eidx) :
+    ∃ val, LamThmValid (lval.insertEVarAt (s.mkFuncsRev lctx) val eidx) lctx (.app s p (LamTerm.bvarApps (.etom eidx) lctx 0)) := by
+    have ⟨hSucc, ⟨wft, ht⟩⟩ := LamThmValidD.ofLamThmValid vt
+    cases wft; case ofApp HArg HFn => cases HFn; case ofBase Hb => cases Hb; case ofExistE =>
+      dsimp [LamWF.interp, LamBaseTerm.LamWF.interp, existLiftFn] at ht;
+      have ⟨valPre, hvalPre⟩ := choose_spec' ht
+      exists LamSort.curryRev valPre; apply LamThmValid.ofLamThmValidD; apply And.intro;
+      case left =>
+        dsimp [LamTerm.maxLooseBVarSucc]; rw [Nat.max_le]; apply And.intro (Nat.max_le.mp hSucc).right
+        apply Nat.le_trans LamTerm.maxLooseBVarSucc_bvarApps; rw [Nat.max_le]
+        apply And.intro (Nat.zero_le _) .refl
+      case right =>
+        let ltv₁ := lval.toLamTyVal
+        let ltv₂ := { lval.toLamTyVal with lamEVarTy := replaceAt (s.mkFuncsRev lctx) eidx lval.lamEVarTy}
+        have HArg' := LamWF.eVarIrrelevance (ltv₁:=ltv₁) (ltv₂:=ltv₂) rfl rfl
+          (fun n H => LamTyVal.insertEVarAt_eVarIrrelevance (Nat.le_trans H heVar)) HArg
+        exists (.ofApp _ HArg' (LamWF.bvarApps (ex:=[]) LamWF.insertEVarAt_eIdx))
+        intro lctxTerm; dsimp [LamWF.interp]
+        apply Eq.mp _ (hvalPre lctxTerm); apply congrArg; apply eq_of_heq
+        apply congr_hd_heq <;> try rfl
+        case h₁ =>
+          apply LamWF.interp_eVarIrrelevance <;> try rfl;
+          intros n H; apply LamValuation.insertEVarAt_eVarIrrelevance;
+          apply Nat.le_trans H heVar
+        case h₂ =>
+          apply HEq.symm
+          apply LamWF.interp_bvarApps (tyex:=[]) (termex:=.nil) LamWF.insertEVarAt_eIdx
+          apply LamWF.interp_insertEVarAt_eIdx
+
+  theorem LamThmValid.skolemize?
+    (vt : LamThmValid lval lctx t) (heq : t.skolemize? eidx lctx = .some (s, t'))
+    (heVar : t.maxEVarSucc ≤ eidx) :
+    ∃ val, LamThmValid (lval.insertEVarAt (s.mkFuncsRev lctx) val eidx) lctx t' := by
+    have ⟨_, ⟨wft, ht⟩⟩ := LamThmValidD.ofLamThmValid vt
+    match t, heq with
+    | .app _ (.base (.existE s)) p, Eq.refl _ =>
+      match wft with
+      | .ofApp _ (.ofBase (.ofExistE _)) HArg =>
+        dsimp [LamTerm.maxEVarSucc] at heVar; rw [Nat.max_le] at heVar
+        apply LamThmValid.skolemize vt heVar.right
+
+end Skolemization
+
+end Auto.Embedding.Lam
