Auto/Embedding/LamLCtx.lean
@@ -1,0 +1,106 @@
+import Auto.Embedding.LamSystem
+
+namespace Auto.Embedding.Lam
+
+def LamTerm.intro1F? (t : LamTerm) : Option (LamSort × LamTerm) :=
+  match t with
+  | .app _ (.base (.forallE s)) (.lam _ t) => .some (s, t)
+  | _ => .none
+
+theorem LamTerm.maxEVarSucc_intro1F?
+  (heq : LamTerm.intro1F? t = .some (s, t')) : t'.maxEVarSucc = t.maxEVarSucc :=
+  match t, heq with
+  | .app _ (.base (.forallE _)) (.lam _ _), Eq.refl _ => by
+    simp [maxEVarSucc, Nat.max, Nat.max_zero_left]
+
+theorem LamValid.intro1F? (H : LamValid lval lctx t)
+  (heq : LamTerm.intro1F? t = .some (s, p)) : LamValid lval (pushLCtx s lctx) p :=
+  match t, heq with
+  | .app _ (.base (.forallE _)) (.lam _ _), Eq.refl _ =>
+    have ⟨wfl, _⟩ := H
+    match wfl with
+    | .ofApp _ (.ofBase (.ofForallE _)) (.ofLam _ Hp) => by
+      apply LamValid.intro1F H
+
+-- First-order logic style intro1
+theorem LamThmValid.intro1F? (H : LamThmValid lval lctx t)
+  (heq : LamTerm.intro1F? t = .some (s, p)) : LamThmValid lval (s :: lctx) p :=
+  fun lctx' => by rw [pushLCtxs_cons]; apply LamValid.intro1F? (H lctx') heq
+
+def LamTerm.intro1H? (t : LamTerm) : Option (LamSort × LamTerm) :=
+  match t with
+  | .app _ (.base (.forallE s)) p => .some (s, .app s p.bvarLift (.bvar 0))
+  | _ => .none
+
+theorem LamTerm.maxEVarSucc_intro1H?
+  (heq : LamTerm.intro1H? t = .some (s, t')) : t'.maxEVarSucc = t.maxEVarSucc := by
+  match t, heq with
+  | .app _ (.base (.forallE s)) p, Eq.refl _ =>
+    dsimp [maxEVarSucc, bvarLift, bvarLiftIdx, bvarLiftsIdx];
+    rw [LamTerm.maxEVarSucc_mapBVarAt]; apply Nat.max_comm
+
+theorem LamValid.intro1H? (H : LamValid lval lctx t)
+  (heq : LamTerm.intro1H? t = .some (s, p)) : LamValid lval (pushLCtx s lctx) p :=
+  match t, heq with
+  | .app s' (.base (.forallE s)) t, Eq.refl _ =>
+    have ⟨wfl, vl⟩ := H
+    match wfl with
+    | .ofApp _ (.ofBase (.ofForallE _)) Hp => by
+      let Hp' := LamWF.ofBVarLiftIdx (s:=s) 0 _ Hp
+      let HApp := LamWF.ofApp s Hp' (.ofBVar 0)
+      rw [← pushLCtxAt_zero]; exists HApp; intro lctxTerm
+      dsimp [LamWF.interp]
+      have vl' := vl (fun n => lctxTerm (.succ n)) (lctxTerm 0)
+      apply Eq.mp _ vl'; apply congrArg; apply congrFun;
+      apply Eq.trans (LamWF.interp_ofBVarLiftIdx lval (idx:=0) lctx
+        (fun n => lctxTerm (Nat.succ n)) (lctxTerm 0) _ Hp) ?req
+      apply eq_of_heq; apply LamWF.interp_heq <;> try rfl
+      case HLCtxTermEq =>
+        apply HEq.funext; intro n; cases n <;> rfl
+
+-- Higher-order logic style intro1
+theorem LamThmValid.intro1H? (H : LamThmValid lval lctx t)
+  (heq : LamTerm.intro1H? t = .some (s, p)) : LamThmValid lval (s :: lctx) p :=
+  fun lctx' => by rw [pushLCtxs_cons]; apply LamValid.intro1H? (H lctx') heq
+
+def LamTerm.intro1? (t : LamTerm) : Option (LamSort × LamTerm) :=
+  match t with
+  | .app _ (.base (.forallE s)) p =>
+    match p with
+    | .lam _ t => .some (s, t)
+    | _ => .some (s, .app s p.bvarLift (.bvar 0))
+  | _ => .none
+
+theorem LamTerm.maxEVarSucc_intro1? (heq : LamTerm.intro1? t = .some (s, t')) :
+  t'.maxEVarSucc = t.maxEVarSucc := by
+  cases t <;> try cases heq
+  case app _ fn p =>
+    cases fn <;> try cases heq
+    case base b =>
+      cases b <;> try cases heq
+      case forallE s =>
+        dsimp [intro1?] at heq;
+        dsimp [maxEVarSucc]; rw [Nat.max, Nat.max_def]; simp [Nat.zero_le]
+        cases p <;> cases heq <;> try rfl
+        case app.refl =>
+          dsimp [maxEVarSucc]; rw [LamTerm.maxEVarSucc_mapBVarAt]; rw [LamTerm.maxEVarSucc_mapBVarAt]
+          rw [Nat.max, Nat.max_comm, Nat.max_def]; simp [Nat.zero_le]
+
+theorem LamValid.intro1? (H : LamValid lval lctx t)
+  (heq : LamTerm.intro1? t = .some (s, p)) : LamValid lval (pushLCtx s lctx) p := by
+  dsimp [LamTerm.intro1?] at heq
+  cases t <;> try cases heq
+  case app _ fn p =>
+    cases fn <;> try cases heq
+    case base b =>
+      cases b <;> try cases heq
+      case forallE s =>
+        dsimp at heq
+        cases p <;> try apply LamValid.intro1H? H heq
+        apply LamValid.intro1F? H heq
+
+theorem LamThmValid.intro1? (H : LamThmValid lval lctx t)
+  (heq : LamTerm.intro1? t = .some (s, p)) : LamThmValid lval (s :: lctx) p :=
+  fun lctx' => by rw [pushLCtxs_cons]; apply LamValid.intro1? (H lctx') heq
+
+end Auto.Embedding.Lam
